wip

Matroid/Constructions/ModularSum.lean
@@ -62,16 +62,19 @@ lemma IsSummablePair.closure_inter_eq_closure (h : IsSummablePair M N T) (hX : X
     M.restrict_closure_eq hX (by grind),
     inter_eq_self_of_subset_left (h.isModularFlat_left.isFlat.closure_subset_of_subset hX)]
 
--- lemma IsSummablePair.closure_inter_subset (h : IsSummablePair M N T) :
---     M.closure X ∩ T ⊆ M.closure X := by
---   rw [← N.closure_inter_ground]
-
-
 lemma IsSummablePair.closure_subset_closure (h : IsSummablePair M N T) (hX : X ⊆ N.E) :
     M.closure X ⊆ N.closure X := by
   wlog hXT : X ⊆ T generalizing X with aux
   · grw [← closure_inter_ground, aux (by grind) (by grind), inter_subset_left]
   grw [← h.closure_inter_eq_closure hXT, inter_subset_left]
+
+lemma IsSummablePair.closure_union_inter_subset_closure (h : IsSummablePair M N T) (hY : Y ⊆ N.E) :
+    M.closure (X ∪ Y) ∩ T ⊆ N.closure ((M.closure X ∩ T) ∪ Y) := by
+  grw [← M.closure_union_closure_left_eq, inter_comm,
+    ← M.closure_union_congr_right (M.closure_inter_ground ..),
+    h.isModularFlat_left.distrib_of_subset_self
+    (M.closure_isFlat ..) (by grind), h.closure_subset_closure (by grind),
+    inter_subset_left (t := M.E), inter_comm]
 
 lemma IsSummablePair.isFlat_left_closure_right_inter (h : IsSummablePair M N T) (X : Set α) :
     M.IsFlat (N.closure X ∩ M.E) := by
@@ -87,96 +90,240 @@ lemma IsSummablePair.isFlat_left_closure_right_inter (h : IsSummablePair M N T) 
 
 lemma IsSummablePair.closure_union_inter_subset (h : IsSummablePair M N T) (X : Set α) :
     M.closure (X ∪ N.closure X) ∩ T ⊆ N.closure (X ∪ M.closure X) := by
-  grw [h.closure_union_closure_right, ← closure_union_closure_left_eq, inter_comm _ T,
-    h.isModularFlat_left.distrib_of_subset_self (M.closure_isFlat ..) (by grind),
-    h.closure_subset_closure (by grind), union_comm]
-  refine closure_subset_closure_of_subset_closure <| union_subset ?_ ?_
-  · grw [← subset_union_left, inter_subset_left]
-  grw [← subset_union_right, N.subset_closure (T ∩ M.closure X) (by grind), inter_subset_right]
-
+  grw [← M.closure_union_congr_right (M.closure_inter_ground ..),
+    h.closure_union_inter_subset_closure (by grind), union_comm,
+    inter_subset_left, N.closure_union_closure_left_eq, inter_subset_left]
 
 def biclosure (M N : Matroid α) (X : Set α) : Set α :=
-  M.closure (X ∪ N.closure X) ∪ N.closure (X ∪ M.closure X)
+  M.closure (X ∪ N.closure (X ∪ M.closure X)) ∪ N.closure (X ∪ M.closure X)
 
 lemma biclosure_subset_biclosure (M N : Matroid α) (hXY : X ⊆ Y) :
     biclosure M N X ⊆ biclosure M N Y := by
   grw [biclosure, hXY, ← biclosure]
 
 lemma subset_biclosure (M N : Matroid α) (hX : X ⊆ M.E ∪ N.E) : X ⊆ biclosure M N X := by
-  rw [biclosure, ← inter_eq_self_of_subset_left hX, inter_union_distrib_left]
-  refine union_subset_union ?_ ?_
-  · grw [← subset_union_left, ← subset_union_left, ← M.subset_closure ..]
-  grw [← subset_union_left, ← subset_union_right, ← N.subset_closure ..]
+  nth_grw 1 [biclosure, ← inter_eq_self_of_subset_left hX, inter_union_distrib_left]
+  apply union_subset_union <;>
+  grw [← subset_union_left, inter_ground_subset_closure]
 
 lemma biclosure_subset_union_ground (M N : Matroid α) (X : Set α) :
     biclosure M N X ⊆ M.E ∪ N.E :=
   union_subset_union (closure_subset_ground ..) (closure_subset_ground ..)
 
+lemma biclosure_inter_union_ground (M N : Matroid α) (X : Set α) :
+    biclosure M N (X ∩ (M.E ∪ N.E)) = biclosure M N X := by
+  rw [biclosure, biclosure]
+  convert rfl using 2
+  · rw [eq_comm, ← M.closure_inter_ground, union_inter_distrib_right,
+      ← M.closure_inter_ground (X ∩ _), inter_assoc, inter_eq_self_of_subset_right
+      subset_union_left, ← N.closure_inter_ground, union_inter_distrib_right,
+      inter_assoc, inter_eq_self_of_subset_right subset_union_right,
+      ← union_inter_distrib_right, ← union_inter_distrib_right, closure_inter_ground,
+      closure_inter_ground, closure_inter_ground]
+  rw [eq_comm, ← N.closure_inter_ground, union_inter_distrib_right, inter_assoc,
+    inter_eq_self_of_subset_right subset_union_right, ← union_inter_distrib_right,
+    closure_inter_ground, ← M.closure_inter_ground, inter_assoc,
+    inter_eq_self_of_subset_right subset_union_left, closure_inter_ground]
+
+lemma biclosure_inter_inter_ground (M N : Matroid α) (X : Set α) :
+    biclosure M N (X ∩ (M.E ∪ N.E)) ∩ (M.E ∪ N.E) = biclosure M N X := by
+  grw [biclosure_inter_union_ground, inter_eq_left, biclosure_subset_union_ground ..]
+
 lemma IsSummablePair.biclosure_inter_right_eq (h : IsSummablePair M N T) (X : Set α) :
     (biclosure M N X) ∩ N.E = N.closure (X ∪ M.closure X) := by
-  grw [biclosure, union_inter_distrib_right,
+  nth_grw 1 [biclosure, union_inter_distrib_right,
     inter_eq_self_of_subset_left (N.closure_subset_ground ..), union_eq_right,
-    h.closure_inter_right, h.closure_union_inter_subset]
+    h.closure_inter_right, subset_union_left (s := X) (t := M.closure X),
+    h.closure_union_inter_subset, union_assoc,
+    union_eq_self_of_subset_left (M.closure_subset_closure subset_union_left),
+    Matroid.closure_union_closure_right_eq, union_self]
 
+lemma biclosure_inter_left_eq (M N : Matroid α) (X : Set α) :
+    (biclosure M N X) ∩ M.E = M.closure (X ∪ N.closure (X ∪ M.closure X)) := by
+  grw [biclosure, union_inter_distrib_right,
+    inter_eq_self_of_subset_left (M.closure_subset_ground _), union_eq_left,
+    M.inter_ground_subset_closure, ← subset_union_right (s := X) (t := N.closure _)]
 
--- lemma IsSummablePair.foo (h : IsSummablePair M N T) (X : Set α) :
---     M.closure (N.closure (X ∪ M.closure X)) ⊆ M.closure (N.closure X) := by
---   refine closure_subset_closure_of_subset_closure ?_
+lemma closure_biclosure_left (X : Set α) : M.closure (biclosure M N X) = biclosure M N X ∩ M.E := by
+  refine (M.inter_ground_subset_closure _).antisymm' ?_
+  rw [biclosure_inter_left_eq, ← M.closure_inter_ground]
+  refine M.closure_subset_closure_of_subset_closure <| ?_
+  grw [biclosure, union_inter_distrib_right, union_subset_iff, and_iff_right inter_subset_left,
+    M.inter_ground_subset_closure, ← subset_union_right (s := X) (t := N.closure _)]
 
-lemma IsSummablePair.closure_biclosure (h : IsSummablePair M N T) :
-    M.closure (biclosure M N X) = (biclosure M N X) ∩ M.E := by
-  refine (subset_inter ?_ (M.closure_subset_ground _)).antisymm
-    <| inter_ground_subset_closure ..
-  rw [biclosure, closure_union_closure_left_eq, union_assoc,
-    union_eq_self_of_subset_left (N.closure_subset_closure subset_union_left),
-    ← closure_union_closure_left_eq, ← M.closure_union_closure_left_eq X,
-    ← N.closure_union_closure_left_eq]
-  set F := M.closure X with hF
-  set G := N.closure X with hG
-  rw [← M.closure_inter_ground, union_inter_distrib_right,
-    inter_eq_self_of_subset_left (show F ⊆ M.E from M.closure_subset_ground ..),
-    h.closure_inter_left, union_comm G]
-  have hmod := h.isModularFlat_left.distrib_of_subset_self (X := F) (Y := N.closure (F ∪ G) ∩ T)
-    (M.closure_isFlat ..) inter_subset_right
-  intro e he
-  by_cases heT : e ∈ T
-  · refine mem_of_mem_of_subset (hmod.subset ⟨heT, he⟩) ?_
-    grw [h.closure_subset_closure (by grind), ← subset_union_right (s := M.closure (F ∪ G)),
-      union_eq_self_of_subset_left, inter_subset_left, closure_closure]
-    grw [subset_inter_iff, and_iff_left inter_subset_left, ← subset_union_left,
-      hF, inter_comm, ← h.closure_inter_right, inter_ground_subset_closure]
-  left
-
-  have P : Set α := sorry
-  have Q : Set α := sorry
-  have' := h.isModularFlat_left.distrib_of_subset_self (X := P) (Y := Q)
-    -- union_comm, inter_comm _ T, ← inter_self T, inter_assoc]
-  -- have' := (h.isModularFlat_left.isModularPair (F := F) (M.closure_isFlat X)).distrib_of_subset_left
-  --   (Y := N.closure (F ∪ G) ∩ T) (h.isModularFlat_left.isFlat) inter_subset_right
-
-  -- have' := h.isModularFlat_left.distrib_of_subset_self (Y := N.closure (F ∪ G) ∩ T) (X := F)
-  --   (closure_isFlat ..) inter_subset_right
-
-  -- (h.isFlat_left_closure_right_inter (F ∪ G))
-
-
-
-
-  -- rw [biclosure]
+lemma IsSummablePair.closure_biclosure_right (h : IsSummablePair M N T) (X : Set α) :
+    N.closure (biclosure M N X) = biclosure M N X ∩ N.E := by
+  refine (N.inter_ground_subset_closure _).antisymm' ?_
+  rw [h.biclosure_inter_right_eq, ← N.closure_inter_ground]
+  exact N.closure_subset_closure_of_subset_closure <| by rw [h.biclosure_inter_right_eq]
 
 lemma IsSummablePair.biclosure_biclosure (h : IsSummablePair M N T) (X : Set α) :
     biclosure M N (biclosure M N X) = biclosure M N X := by
-  refine subset_antisymm ?_ (subset_biclosure _ _ (biclosure_subset_union_ground ..))
-  nth_rw 1 [biclosure, ← N.closure_inter_ground, h.biclosure_inter_right_eq, N.closure_closure,
-    biclosure, union_assoc, union_self, ← biclosure, ← N.closure_inter_ground,
-      union_inter_distrib_right, h.biclosure_inter_right_eq, N.closure_union_closure_left_eq,
+  refine (subset_biclosure _ _ (biclosure_subset_union_ground ..)).antisymm' ?_
+  grw [biclosure, closure_biclosure_left, union_eq_self_of_subset_right inter_subset_left,
+    h.closure_biclosure_right, union_eq_self_of_subset_right inter_subset_left,
+    closure_biclosure_left, ← inter_union_distrib_left, inter_subset_left]
+
+-- (closure_exchange : ∀ ⦃X e f⦄, X ⊆ E → e ∈ E → f ∈ E →
+--       f ∈ closure (insert e X) \ closure X → e ∈ closure (insert f X) \ X)
+
+lemma IsSummablePair.biclosure_biclosure_insert (h : IsSummablePair M N T) (hX : X ⊆ M.E ∪ N.E)
+    (he : e ∈ M.E ∪ N.E) :
+    M.biclosure N (insert e (M.biclosure N X)) = M.biclosure N (insert e X) := by
+  refine subset_antisymm ?_ <| biclosure_subset_biclosure _ _ <| insert_subset_insert <|
+    subset_biclosure _ _ hX
+  nth_rw 3 [← h.biclosure_biclosure]
+  refine biclosure_subset_biclosure _ _ <| insert_subset ?_ <| biclosure_subset_biclosure _ _
+    <| subset_insert ..
+  grw [← subset_biclosure _ _ (insert_subset he hX)]
+  exact mem_insert ..
+
+-- FALSE
+lemma IsSummablePair.closure_inter_biclosure_left (h : IsSummablePair M N T) (hX : X ⊆ M.E ∪ N.E)
+    (he : e ∈ M.E) : M.closure (insert e (M.biclosure N X)) = biclosure M N (insert e X) ∩ M.E := by
+  refine subset_antisymm ?_ ?_
+  · grw [← h.biclosure_biclosure_insert hX (.inl he), biclosure_inter_left_eq, ← subset_union_left]
+  rw [← M.closure_inter_ground, insert_inter_of_mem he, biclosure_inter_left_eq,
+    biclosure_inter_left_eq, closure_insert_closure_eq_closure_insert,
+    insert_union (t := M.closure _), ← union_insert,
+    insert_eq_of_mem (M.mem_closure_of_mem' (mem_insert ..) he)]
+  obtain heq | hssu :=
+    (inter_subset_inter_left N.E (M.closure_subset_closure (subset_insert e X))).eq_or_ssubset
+  · rw [← closure_union_congr_right (N.closure_inter_ground ..),
+      ← heq, closure_union_congr_right (N.closure_inter_ground ..), insert_union]
+  obtain ⟨f, ⟨hfeX, hfN⟩, hfX⟩ := exists_of_ssubset hssu
+  rw [mem_inter_iff, and_iff_left hfN] at hfX
+  have hss : N.closure (M.closure (insert e X)) ⊆ N.closure (insert f (M.closure X)) := by
+    grw [← closure_insert_congr ⟨hfeX, hfX⟩, ← N.closure_inter_ground,
+      closure_subset_closure_iff_subset_closure, h.closure_inter_right, ← union_singleton,
+      h.closure_union_inter_subset_closure (by simpa), ← union_singleton, inter_subset_left]
+  have aux : Disjoint X M.E := sorry
+  rw [← closure_inter_ground, union_inter_distrib_right, ← M.closure_inter_ground (insert e X),
+    ← M.closure_inter_ground X, insert_inter_of_mem he, aux.inter_eq]
+  simp
+  have hss2 : M.closure (N.closure (insert f (X ∪ M.closure X))) ⊆
+      M.closure (insert f (N.closure (X ∪ M.closure X))) := by
+    rw [← M.closure_inter_ground]
+    refine closure_subset_closure_of_subset_closure ?_
+    rw [← N.closure_insert_closure_eq_closure_insert]
+    sorry
+  grw [← N.closure_union_closure_right_eq, hss, N.closure_union_closure_right_eq, union_insert,
+    ← M.closure_union_closure_right_eq, hss2, M.closure_union_closure_right_eq]
+    -- rw [h.clo]
 
 
-      h.closure_biclosure, h.closure_biclosure, union_subset_iff,
-      and_iff_right inter_subset_left, inter_right_comm, h.biclosure_inter_right_eq,
-      ← closure_union_closure_left_eq, union_eq_self_of_subset_right inter_subset_left,
-      closure_closure]
-  exact subset_union_right
+  -- rw [← closure_insert_congr ⟨hfeX, hfX⟩, closure_union_congr_right (N.closure_inter_ground ..)]
+  -- have := (M.closure_exchange ⟨hfeX, hfX⟩).1
+  -- grw [biclosure_inter_left_eq]
+  -- rw [← closure_biclosure_left]
+  -- rw [← inter_eq_self_of_subset_left (M.closure_subset_ground ..)]
+
+lemma IsSummablePair.closure_exchange (h : IsSummablePair M N T) (hX : X ⊆ M.E ∪ N.E)
+    (he : e ∈ M.E ∪ N.E) (hf : f ∈ M.E ∪ N.E) (hfX : f ∉ M.biclosure N X)
+    (hfeX : f ∈ M.biclosure N (insert e X)) : e ∈ M.biclosure N (insert f X) := by
+  rw [← h.biclosure_biclosure_insert hX hf]
+  obtain hfE | hfE := hf
+  · have h1 := mem_inter hfeX hfE
+    rw [biclosure_inter_left_eq] at h1
+    have hins : f ∈ M.closure (insert e (M.biclosure N X)) := by
+      _
+
+  -- suffices hcl' : f ∈ M.closure (insert e (M.biclosure N X))
+  -- ·
+  --   refine mem_of_mem_of_subset (M.closure_exchange ⟨hcl', by grind [closure_biclosure_left]⟩).1 ?_
+  --     grw [← inter_subset_left (s := M.biclosure N (insert f X)) (t := M.E),
+  --       ← closure_inter_ground, insert_inter_of_mem hfE, biclosure_inter_left_eq,
+  --       closure_insert_closure_eq_closure_insert, biclosure_inter_left_eq]
+  --     exact M.closure_subset_closure <| insert_subset (by grind) <| by grw [← subset_insert]
+  by_cases! hfE : f ∉ N.E
+  · have hi := mem_inter hfeX (show f ∈ M.E by grind)
+    rw [biclosure_inter_left_eq] at hi
+    by_cases! heE : e ∉ N.E
+    · rw [← N.closure_inter_ground, union_inter_distrib_right, insert_inter_of_notMem heE,
+        ← union_inter_distrib_right, N.closure_inter_ground] at hi
+      have hins : f ∈ M.closure (insert e (M.biclosure N X)) := by
+        refine mem_of_mem_of_subset hi ?_
+        grw [biclosure, ← subset_union_left (s := M.closure _),
+          closure_insert_closure_eq_closure_insert]
+      refine mem_of_mem_of_subset (M.closure_exchange ⟨hins, by grind [closure_biclosure_left]⟩).1 ?_
+      grw [← inter_subset_left (s := M.biclosure N (insert f X)) (t := M.E),
+        ← closure_inter_ground, insert_inter_of_mem (by grind), biclosure_inter_left_eq,
+        closure_insert_closure_eq_closure_insert, biclosure_inter_left_eq]
+      exact M.closure_subset_closure <| insert_subset (by grind) <| by grw [← subset_insert]
+    rw [← h.biclosure_inter_right_eq] at hi
+      -- have := (M.closure_exchange ⟨hins, ?_⟩).1
+      -- rw [← closure_inter_ground, insert_inter_of_mem (by grind), biclosure_inter_left_eq] at this ⊢
+      -- refine mem_of_mem_of_subset ?_ subset_union_left
+
+
+
+
+
+    -- have hcl := (M.biclosure_inter_left_eq N (insert e X)).subset ⟨hfeX, hfE⟩
+    suffices hcl' : f ∈ M.closure (insert e (M.biclosure N X))
+    · refine mem_of_mem_of_subset (M.closure_exchange ⟨hcl', by grind [closure_biclosure_left]⟩).1 ?_
+      grw [← inter_subset_left (s := M.biclosure N (insert f X)) (t := M.E),
+        ← closure_inter_ground, insert_inter_of_mem hfE, biclosure_inter_left_eq,
+        closure_insert_closure_eq_closure_insert, biclosure_inter_left_eq]
+      exact M.closure_subset_closure <| insert_subset (by grind) <| by grw [← subset_insert]
+    -- refine mem_of_mem_of_subset (mem_inter hfeX hfE) ?_
+    -- rw [biclosure_inter_left_eq]
+    by_cases! heE : e ∉ M.E
+    · have hcon := mem_inter hfeX hfE
+      rw [biclosure_inter_left_eq, ← M.closure_inter_ground, union_inter_distrib_right,
+        ← M.closure_inter_ground (insert ..), insert_inter_of_notMem heE,
+        M.closure_inter_ground, ← union_inter_distrib_right, M.closure_inter_ground] at hcon
+      rw [← closure_inter_ground, insert_inter_of_notMem heE, biclosure_inter_left_eq,
+        closure_closure]
+
+    sorry
+
+    rw [← closure_inter_ground, union_inter_distrib_right, ← M.closure_inter_ground (insert e X),
+      insert_inter_of_notMem heE, closure_inter_ground, ← M.closure_inter_ground (insert e _),
+      insert_inter_of_notMem heE]
+    by_cases heE : e ∈ M.E
+    · refine mem_of_mem_of_subset (mem_inter hfeX hfE) ?_
+      rw [biclosure_inter_left_eq, ← M.closure_inter_ground (insert e (M.biclosure N _)),
+        insert_inter_of_mem heE, biclosure_inter_left_eq, closure_insert_closure_eq_closure_insert,
+        insert_union (t := M.closure (insert e X)), ← union_insert,
+        insert_eq_of_mem (M.mem_closure_of_mem' (mem_insert ..) heE),]
+      sorry
+    rw [← closure_inter_ground, insert_inter_of_notMem heE]
+    refine mem_of_mem_of_subset (mem_inter hfeX hfE) ?_
+
+    obtain heE | heE := he
+    · refine mem_of_mem_of_subset (mem_inter hfeX hfE) ?_
+      rw [biclosure_inter_left_eq, ← M.closure_inter_ground (insert e (M.biclosure N _)),
+        insert_inter_of_mem heE, biclosure_inter_left_eq, closure_insert_closure_eq_closure_insert,
+        insert_union (t := M.closure (insert e X)), ← union_insert,
+        insert_eq_of_mem (M.mem_closure_of_mem' (mem_insert ..) heE)]
+  sorry
+
+
+
+    --   have aux : (N.closure (insert e X ∪ M.closure (insert e X))) ∩ M.E ⊆
+    --       M.closure (insert e (N.closure (X ∪ M.closure X))) := by
+    --     rw [← M.closure_insert_closure_eq_closure_insert (X := N.closure (X ∪ M.closure X))]
+    --   refine M.closure_subset_closure_of_subset_closure ?_
+    --   -- refine closure_subset_closure_of_subset_closure <| union_subset ?_ ?_
+    --   -- · grw [inter_ground_subset_closure, ← ]
+
+    --   -- grw [← closure_inter_ground, insert_inter_of_mem heE, biclosure_inter_left_eq,
+    --   --   closure_insert_closure_eq_closure_insert]
+
+    -- refine mem_of_mem_of_subset (mem_inter hfeX hfE) ?_
+    -- grw [biclosure_inter_left_eq, ← closure_inter_ground, union_inter_distrib_right]
+    -- refine M.closure_subset_closure_of_subset_closure <| union_subset ?_ ?_
+    -- · grw [inter_ground_subset_closure, ← subset_biclosure _ _ hX]
+    -- grw [inter_ground_subset_closure]
+    -- sorry
+
+    -- grw [← closure_insert_closure_eq_closure_insert, closure_biclosure_left,
+    --   biclosure_inter_left_eq, closure_insert_closure_eq_closure_insert,
+    --   ← insert_inter_of_mem hfE, closure_inter_ground,
+    --   ← inter_subset_left (s := M.biclosure N (insert f X)) (t := M.E),
+    --   biclosure_inter_left_eq]
+    -- refine closure_subset_closure_of_subset_closure ?_
 
 
 
@@ -185,246 +332,246 @@ lemma IsSummablePair.biclosure_biclosure (h : IsSummablePair M N T) (X : Set α)
 
 
 
-structure IsFlatPair (M N : Matroid α) (F₀ F₁ : Set α) where
-  isFlat_left : M.IsFlat F₀
-  isFlat_right : N.IsFlat F₁
-  subset_right : F₀ ∩ N.E ⊆ F₁
-  subset_left : F₁ ∩ M.E ⊆ F₀
+-- structure IsFlatPair (M N : Matroid α) (F₀ F₁ : Set α) where
+--   isFlat_left : M.IsFlat F₀
+--   isFlat_right : N.IsFlat F₁
+--   subset_right : F₀ ∩ N.E ⊆ F₁
+--   subset_left : F₁ ∩ M.E ⊆ F₀
 
-lemma IsFlatPair.symm (h : IsFlatPair M N F₀ F₁) : IsFlatPair N M F₁ F₀ :=
-  ⟨h.isFlat_right, h.isFlat_left, h.subset_left, h.subset_right⟩
+-- lemma IsFlatPair.symm (h : IsFlatPair M N F₀ F₁) : IsFlatPair N M F₁ F₀ :=
+--   ⟨h.isFlat_right, h.isFlat_left, h.subset_left, h.subset_right⟩
 
-@[grind →]
-lemma IsFlatPair.subset_ground_left (h : IsFlatPair M N F₀ F₁) : F₀ ⊆ M.E :=
-  h.isFlat_left.subset_ground
+-- @[grind →]
+-- lemma IsFlatPair.subset_ground_left (h : IsFlatPair M N F₀ F₁) : F₀ ⊆ M.E :=
+--   h.isFlat_left.subset_ground
 
-@[grind →]
-lemma IsFlatPair.subset_ground_right (h : IsFlatPair M N F₀ F₁) : F₁ ⊆ N.E :=
-  h.isFlat_right.subset_ground
+-- @[grind →]
+-- lemma IsFlatPair.subset_ground_right (h : IsFlatPair M N F₀ F₁) : F₁ ⊆ N.E :=
+--   h.isFlat_right.subset_ground
 
-lemma IsFlatPair.union_inter_ground_left (h : IsFlatPair M N F₀ F₁) : (F₀ ∪ F₁) ∩ M.E = F₀ := by
-  rw [union_inter_distrib_right, inter_eq_self_of_subset_left h.subset_ground_left,
-    union_eq_self_of_subset_right h.subset_left]
+-- lemma IsFlatPair.union_inter_ground_left (h : IsFlatPair M N F₀ F₁) : (F₀ ∪ F₁) ∩ M.E = F₀ := by
+--   rw [union_inter_distrib_right, inter_eq_self_of_subset_left h.subset_ground_left,
+--     union_eq_self_of_subset_right h.subset_left]
 
-lemma IsFlatPair.union_inter_ground_right (h : IsFlatPair M N F₀ F₁) : (F₀ ∪ F₁) ∩ N.E = F₁ := by
-  rw [union_inter_distrib_right, inter_eq_self_of_subset_left h.subset_ground_right,
-    union_eq_self_of_subset_left h.subset_right]
+-- lemma IsFlatPair.union_inter_ground_right (h : IsFlatPair M N F₀ F₁) : (F₀ ∪ F₁) ∩ N.E = F₁ := by
+--   rw [union_inter_distrib_right, inter_eq_self_of_subset_left h.subset_ground_right,
+--     union_eq_self_of_subset_left h.subset_right]
 
-attribute [grind →] IsFlatPair.isFlat_left IsFlatPair.isFlat_right
+-- attribute [grind →] IsFlatPair.isFlat_left IsFlatPair.isFlat_right
 
-lemma IsSummablePair.isFlatPair (h : IsSummablePair M N T) (hF₀ : M.IsFlat F₀) (X : Set α) :
-    IsFlatPair M N (M.closure (F₀ ∪ N.closure (F₀ ∪ X))) (N.closure (F₀ ∪ X)) := by
-  refine ⟨by simp, by simp, ?_, ?_⟩
-  · grw [h.closure_inter_right, ← closure_inter_ground, union_inter_distrib_right,
-      inter_eq_self_of_subset_left hF₀.subset_ground, h.closure_inter_left, inter_comm,
-      h.isModularFlat_left.distrib_of_subset_self hF₀ (Y := N.closure (F₀ ∪ X) ∩ T)
-      inter_subset_right, h.closure_subset_closure (by grind)]
-    refine N.closure_subset_closure_of_subset_closure <| union_subset ?_ inter_subset_left
-    exact subset_closure_of_subset' _ (by grind) (by grind)
-  grw [← subset_union_right (t := N.closure (F₀ ∪ X)),
-    ← M.subset_closure_of_subset' inter_subset_left inter_subset_right]
+-- lemma IsSummablePair.isFlatPair (h : IsSummablePair M N T) (hF₀ : M.IsFlat F₀) (X : Set α) :
+--     IsFlatPair M N (M.closure (F₀ ∪ N.closure (F₀ ∪ X))) (N.closure (F₀ ∪ X)) := by
+--   refine ⟨by simp, by simp, ?_, ?_⟩
+--   · grw [h.closure_inter_right, ← closure_inter_ground, union_inter_distrib_right,
+--       inter_eq_self_of_subset_left hF₀.subset_ground, h.closure_inter_left, inter_comm,
+--       h.isModularFlat_left.distrib_of_subset_self hF₀ (Y := N.closure (F₀ ∪ X) ∩ T)
+--       inter_subset_right, h.closure_subset_closure (by grind)]
+--     refine N.closure_subset_closure_of_subset_closure <| union_subset ?_ inter_subset_left
+--     exact subset_closure_of_subset' _ (by grind) (by grind)
+--   grw [← subset_union_right (t := N.closure (F₀ ∪ X)),
+--     ← M.subset_closure_of_subset' inter_subset_left inter_subset_right]
 
-def IsSumFlat (M N : Matroid α) (F : Set α) : Prop :=
-  ∃ F₀ F₁, IsFlatPair M N F₀ F₁ ∧ F₀ ∪ F₁ = F
+-- def IsSumFlat (M N : Matroid α) (F : Set α) : Prop :=
+--   ∃ F₀ F₁, IsFlatPair M N F₀ F₁ ∧ F₀ ∪ F₁ = F
 
-lemma IsSumFlat.symm (h : IsSumFlat M N F) : IsSumFlat N M F := by
-  obtain ⟨F₀, F₁, h, rfl⟩ := h
-  exact ⟨F₁, F₀, h.symm, union_comm ..⟩
+-- lemma IsSumFlat.symm (h : IsSumFlat M N F) : IsSumFlat N M F := by
+--   obtain ⟨F₀, F₁, h, rfl⟩ := h
+--   exact ⟨F₁, F₀, h.symm, union_comm ..⟩
 
-lemma IsFlatPair.isSumFlat_union (h : IsFlatPair M N F₀ F₁) : IsSumFlat M N (F₀ ∪ F₁) :=
-  ⟨_, _, h, rfl⟩
+-- lemma IsFlatPair.isSumFlat_union (h : IsFlatPair M N F₀ F₁) : IsSumFlat M N (F₀ ∪ F₁) :=
+--   ⟨_, _, h, rfl⟩
 
--- /-- If `F` is a sum flat containing the flat `F₀` on the LHS and the set `X` on the RHS,
--- then it must contain a bunch of other stuff. -/
--- lemma IsSumFlat.subset_of_subset_subset (h : M.IsSumFlat N F) (hF₀ : M.IsFlat F₀) (hF₀F : F₀ ⊆ F)
---     (hX : X ⊆ N.E) (hXF : X ⊆ F) :
---     M.closure (F₀ ∪ N.closure (F₀ ∪ X)) ∪ N.closure (F₀ ∪ X) ⊆ F := by
+-- -- /-- If `F` is a sum flat containing the flat `F₀` on the LHS and the set `X` on the RHS,
+-- -- then it must contain a bunch of other stuff. -/
+-- -- lemma IsSumFlat.subset_of_subset_subset (h : M.IsSumFlat N F) (hF₀ : M.IsFlat F₀) (hF₀F : F₀ ⊆ F)
+-- --     (hX : X ⊆ N.E) (hXF : X ⊆ F) :
+-- --     M.closure (F₀ ∪ N.closure (F₀ ∪ X)) ∪ N.closure (F₀ ∪ X) ⊆ F := by
+-- --   obtain ⟨K₀, K₁, hK, rfl⟩ := h
+-- --   have h₀ : F₀ ⊆ K₀ := by
+-- --     rwa [← hK.union_inter_ground_left, subset_inter_iff, and_iff_left hF₀.subset_ground]
+-- --   have hss : N.closure (F₀ ∪ X) ⊆ K₁ := by
+-- --     grw [← closure_inter_ground, union_inter_distrib_right, inter_eq_self_of_subset_left hX]
+-- --     refine hK.isFlat_right.closure_subset_of_subset <| union_subset ?_ ?_
+-- --     · grw [h₀, ← hK.union_inter_ground_right, ← subset_union_left]
+-- --     grw [← hK.union_inter_ground_right, subset_inter_iff, and_iff_left hX, hXF]
+-- --   refine union_subset_union ?_ hss
+-- --   nth_grw 1 [h₀, hss, ← closure_inter_ground, hK.union_inter_ground_left, hK.isFlat_left.closure]
+
+-- -- lemma IsSumFlat.subset_of_subset_subset' (h : M.IsSumFlat N F) (hXF : X ⊆ F) (hYF : Y ⊆ F) :
+-- --     M.closure (X ∪ N.closure (X ∪ Y)) ⊆ F := by
+-- --   obtain ⟨K₀, K₁, hK, rfl⟩ := h
+-- --   grw [← subset_union_left (s := K₀), hXF, ← closure_inter_ground, union_inter_distrib_right,
+-- --     hK.union_inter_ground_left, union_eq_self_of_subset_right hYF,
+-- --       ← N.closure_inter_ground, hK.union_inter_ground_right, hK.isFlat_right.closure,
+-- --       ← inter_eq_self_of_subset_left hK.subset_ground_left, ← union_inter_distrib_right,
+-- --       hK.union_inter_ground_left, hK.isFlat_left.closure,
+-- --       inter_eq_self_of_subset_left hK.subset_ground_left]
+
+-- lemma IsSumFlat.subset_of_subset_subset (h : M.IsSumFlat N F) (hXF : X ⊆ F) :
+--     M.closure (X ∪ N.closure X) ⊆ F := by
 --   obtain ⟨K₀, K₁, hK, rfl⟩ := h
---   have h₀ : F₀ ⊆ K₀ := by
---     rwa [← hK.union_inter_ground_left, subset_inter_iff, and_iff_left hF₀.subset_ground]
---   have hss : N.closure (F₀ ∪ X) ⊆ K₁ := by
---     grw [← closure_inter_ground, union_inter_distrib_right, inter_eq_self_of_subset_left hX]
---     refine hK.isFlat_right.closure_subset_of_subset <| union_subset ?_ ?_
---     · grw [h₀, ← hK.union_inter_ground_right, ← subset_union_left]
---     grw [← hK.union_inter_ground_right, subset_inter_iff, and_iff_left hX, hXF]
---   refine union_subset_union ?_ hss
---   nth_grw 1 [h₀, hss, ← closure_inter_ground, hK.union_inter_ground_left, hK.isFlat_left.closure]
+--   grw [hXF, ← N.closure_inter_ground, hK.union_inter_ground_right, hK.isFlat_right.closure,
+--     union_assoc, union_self, ← closure_inter_ground, hK.union_inter_ground_left,
+--     hK.isFlat_left.closure, ← subset_union_left]
 
--- lemma IsSumFlat.subset_of_subset_subset' (h : M.IsSumFlat N F) (hXF : X ⊆ F) (hYF : Y ⊆ F) :
---     M.closure (X ∪ N.closure (X ∪ Y)) ⊆ F := by
---   obtain ⟨K₀, K₁, hK, rfl⟩ := h
---   grw [← subset_union_left (s := K₀), hXF, ← closure_inter_ground, union_inter_distrib_right,
---     hK.union_inter_ground_left, union_eq_self_of_subset_right hYF,
---       ← N.closure_inter_ground, hK.union_inter_ground_right, hK.isFlat_right.closure,
---       ← inter_eq_self_of_subset_left hK.subset_ground_left, ← union_inter_distrib_right,
---       hK.union_inter_ground_left, hK.isFlat_left.closure,
---       inter_eq_self_of_subset_left hK.subset_ground_left]
+-- lemma foo (h : IsSummablePair M N T) (h : IsSumFlat M N F) (he : e ∈ M.E) (heF₀ : e ∉ F) :
+--     ∃ (F' : Set α), e ∈ F' ∧ Minimal (fun X ↦ F ⊂ X ∧ IsSumFlat M N X) F' := by
+--   obtain ⟨F₀, F₁, hF₀F₁, rfl⟩ := h
 
-lemma IsSumFlat.subset_of_subset_subset (h : M.IsSumFlat N F) (hXF : X ⊆ F) :
-    M.closure (X ∪ N.closure X) ⊆ F := by
-  obtain ⟨K₀, K₁, hK, rfl⟩ := h
-  grw [hXF, ← N.closure_inter_ground, hK.union_inter_ground_right, hK.isFlat_right.closure,
-    union_assoc, union_self, ← closure_inter_ground, hK.union_inter_ground_left,
-    hK.isFlat_left.closure, ← subset_union_left]
+--   -- have h' := h.isFlatPair (M.closure_isFlat (insert e F₀)) F₁
+--   -- rw [closure_union_closure_left_eq] at h'
 
-lemma foo (h : IsSummablePair M N T) (h : IsSumFlat M N F) (he : e ∈ M.E) (heF₀ : e ∉ F) :
-    ∃ (F' : Set α), e ∈ F' ∧ Minimal (fun X ↦ F ⊂ X ∧ IsSumFlat M N X) F' := by
-  obtain ⟨F₀, F₁, hF₀F₁, rfl⟩ := h
+--   set F₀e := M.closure (insert e F₀) with hF₀e
+--   have hF₀e_flat : M.IsFlat F₀e := closure_isFlat ..
+--   set F₀' := M.closure (F₀e ∪ N.closure (F₀e ∪ F₁)) with hF₀'
+--   set F₁' := N.closure (F₀e ∪ F₁) with hF₁'
+--   -- set F' := F₀' ∪ F₁' with hF'
+--   have hFp : IsFlatPair M N F₀' F₁' := h.isFlatPair hF₀e_flat F₁
+--   have heF' : e ∈ F₀' ∪ F₁' := by
+--     grw [← subset_union_left, hF₀', hF₀e, ← subset_union_left, closure_closure]
+--     exact M.mem_closure_of_mem' (by simp) he
+--   have hssu : F₀ ∪ F₁ ⊂ F₀' ∪ F₁' := sorry
+--   refine ⟨F₀' ∪ F₁', heF', minimal_iff_forall_ssubset.2 ⟨⟨hssu, hFp.isSumFlat_union⟩, ?_⟩⟩
+--   rintro _ hKss ⟨hssK, K₀, K₁, hK, rfl⟩
+--   have hFK₀ : F₀ ⊆ K₀ := by
+--     grw [← hK.union_inter_ground_left, subset_inter_iff, and_iff_left hF₀F₁.subset_ground_left,
+--       ← hssK, ← subset_union_left]
 
-  -- have h' := h.isFlatPair (M.closure_isFlat (insert e F₀)) F₁
-  -- rw [closure_union_closure_left_eq] at h'
+--   by_cases heK₀ : e ∈ K₀
+--   · refine hKss.not_subset <| union_subset ?_ ?_
+--     · grw [← hK.isSumFlat_union.subset_of_subset_subset (X := insert e (F₀ ∪ F₁)) (by grind),
+--         ← subset_union_left, hF₀', ← closure_inter_ground,
+--         closure_subset_closure_iff_subset_closure, union_inter_distrib_right,
+--         inter_eq_self_of_subset_left (by grind), union_subset_iff, hF₀e,
+--         and_iff_right (closure_subset_closure _ (by grind))]
 
-  set F₀e := M.closure (insert e F₀) with hF₀e
-  have hF₀e_flat : M.IsFlat F₀e := closure_isFlat ..
-  set F₀' := M.closure (F₀e ∪ N.closure (F₀e ∪ F₁)) with hF₀'
-  set F₁' := N.closure (F₀e ∪ F₁) with hF₁'
-  -- set F' := F₀' ∪ F₁' with hF'
-  have hFp : IsFlatPair M N F₀' F₁' := h.isFlatPair hF₀e_flat F₁
-  have heF' : e ∈ F₀' ∪ F₁' := by
-    grw [← subset_union_left, hF₀', hF₀e, ← subset_union_left, closure_closure]
-    exact M.mem_closure_of_mem' (by simp) he
-  have hssu : F₀ ∪ F₁ ⊂ F₀' ∪ F₁' := sorry
-  refine ⟨F₀' ∪ F₁', heF', minimal_iff_forall_ssubset.2 ⟨⟨hssu, hFp.isSumFlat_union⟩, ?_⟩⟩
-  rintro _ hKss ⟨hssK, K₀, K₁, hK, rfl⟩
-  have hFK₀ : F₀ ⊆ K₀ := by
-    grw [← hK.union_inter_ground_left, subset_inter_iff, and_iff_left hF₀F₁.subset_ground_left,
-      ← hssK, ← subset_union_left]
+--       -- show K₀ = M.closure (insert e K₀) by rw [insert_eq_of_mem heK₀, hK.isFlat_left.closure],
+--       -- ← hK.isFlat_right.closure,
+--       -- insert_union]
+--     have hss₀ : F₀' ⊆ K₀ := by
+--       -- rw [← hK.union_inter_ground_left, subset_inter_iff, and_iff_left (by grind), ]
+--       grw [hF₀', hF₁', ← closure_inter_ground, hK.isFlat_left.closure_subset_iff_subset (by grind),
+--         union_inter_distrib_right, union_subset_iff,
+--         inter_eq_self_of_subset_left hF₀e_flat.subset_ground, hF₀e,
+--         hK.isFlat_left.closure_subset_iff_subset (by grind), and_iff_right (by grind),
+--         ← hK.union_inter_ground_left, ← insert_eq_self.2 heK₀, insert_union, ← hssK]
+--     have h₀' := hK.isSumFlat_union.subset_of_subset_subset (X := insert e F₀) (by grind)
+--     have h₁' := union_comm K₀ _ ▸ hK.symm.isSumFlat_union.subset_of_subset_subset
+--       (X := F₁) (by grind)
 
-  by_cases heK₀ : e ∈ K₀
-  · refine hKss.not_subset <| union_subset ?_ ?_
-    · grw [← hK.isSumFlat_union.subset_of_subset_subset (X := insert e (F₀ ∪ F₁)) (by grind),
-        ← subset_union_left, hF₀', ← closure_inter_ground,
-        closure_subset_closure_iff_subset_closure, union_inter_distrib_right,
-        inter_eq_self_of_subset_left (by grind), union_subset_iff, hF₀e,
-        and_iff_right (closure_subset_closure _ (by grind))]
+--     refine (h'.trans_ssubset hKss).not_subset ?_
+--     rw [hF₀', hF₁', hF₀e]
 
-      -- show K₀ = M.closure (insert e K₀) by rw [insert_eq_of_mem heK₀, hK.isFlat_left.closure],
-      -- ← hK.isFlat_right.closure,
-      -- insert_union]
-    have hss₀ : F₀' ⊆ K₀ := by
-      -- rw [← hK.union_inter_ground_left, subset_inter_iff, and_iff_left (by grind), ]
-      grw [hF₀', hF₁', ← closure_inter_ground, hK.isFlat_left.closure_subset_iff_subset (by grind),
-        union_inter_distrib_right, union_subset_iff,
-        inter_eq_self_of_subset_left hF₀e_flat.subset_ground, hF₀e,
-        hK.isFlat_left.closure_subset_iff_subset (by grind), and_iff_right (by grind),
-        ← hK.union_inter_ground_left, ← insert_eq_self.2 heK₀, insert_union, ← hssK]
-    have h₀' := hK.isSumFlat_union.subset_of_subset_subset (X := insert e F₀) (by grind)
-    have h₁' := union_comm K₀ _ ▸ hK.symm.isSumFlat_union.subset_of_subset_subset
-      (X := F₁) (by grind)
+--   -- -- set F₀' := M.closure (insert e F₀) with hF₀'
+--   -- -- set F' := M.closure (insert e F₀ ∪ N.closure (F₀e ∪ F₁)) ∪ N.closure (F₀e ∪ F₁) with hF'
+--   -- have heF' : e ∈ F' := .inl <| M.mem_closure_of_mem' (by simp [hF₀e]) he
+--   -- have hssu : F₀ ∪ F₁ ⊂ F' := by
+--   --   refine (union_subset_union ?_ ?_).ssubset_of_mem_notMem heF' heF₀
+--   --   · grw [hF₀', ← subset_union_left, hF₀e, ← subset_insert, hF₀F₁.isFlat_left.closure]
+--   --   grw [hF₁', ← subset_union_right, hF₀F₁.isFlat_right.closure]
+--   -- have := h'.isSumFlat_union
+--   -- simp_rw [minimal_iff_forall_ssubset]
+--   -- refine ⟨F', heF', ⟨hssu, ?_⟩, fun X hXF' ⟨hXssu, hXsf⟩ ↦ ?_⟩
+--   -- · rw [hF', hF₀', hF₁']
+--   -- obtain ⟨K₀, K₁, hK, rfl⟩ := hXsf
+--   -- by_cases heK₀ : e ∈ K₀
+--   -- · have h₀ : F₀' ⊆ K₀ := by
+--   --     grw [hF₀', hK.isFlat_left.closure_subset_iff_subset (by grind), insert_subset_iff,
+--   --       and_iff_right heK₀, ← hK.union_inter_ground_left, ← hF₀F₁.union_inter_ground_left,
+--   --       hXssu]
 
-    refine (h'.trans_ssubset hKss).not_subset ?_
-    rw [hF₀', hF₁', hF₀e]
-
-  -- -- set F₀' := M.closure (insert e F₀) with hF₀'
-  -- -- set F' := M.closure (insert e F₀ ∪ N.closure (F₀e ∪ F₁)) ∪ N.closure (F₀e ∪ F₁) with hF'
-  -- have heF' : e ∈ F' := .inl <| M.mem_closure_of_mem' (by simp [hF₀e]) he
-  -- have hssu : F₀ ∪ F₁ ⊂ F' := by
-  --   refine (union_subset_union ?_ ?_).ssubset_of_mem_notMem heF' heF₀
-  --   · grw [hF₀', ← subset_union_left, hF₀e, ← subset_insert, hF₀F₁.isFlat_left.closure]
-  --   grw [hF₁', ← subset_union_right, hF₀F₁.isFlat_right.closure]
-  -- have := h'.isSumFlat_union
-  -- simp_rw [minimal_iff_forall_ssubset]
-  -- refine ⟨F', heF', ⟨hssu, ?_⟩, fun X hXF' ⟨hXssu, hXsf⟩ ↦ ?_⟩
-  -- · rw [hF', hF₀', hF₁']
-  -- obtain ⟨K₀, K₁, hK, rfl⟩ := hXsf
-  -- by_cases heK₀ : e ∈ K₀
-  -- · have h₀ : F₀' ⊆ K₀ := by
-  --     grw [hF₀', hK.isFlat_left.closure_subset_iff_subset (by grind), insert_subset_iff,
-  --       and_iff_right heK₀, ← hK.union_inter_ground_left, ← hF₀F₁.union_inter_ground_left,
-  --       hXssu]
-
-    -- have h₁ : F₁' ⊆ K₀ := by
+--     -- have h₁ : F₁' ⊆ K₀ := by
 
 
 
-  -- refine ⟨_, ?_, minimal_iff_forall_ssubset.2 ⟨⟨?_, h'.isSumFlat_union⟩, ?_⟩⟩
+--   -- refine ⟨_, ?_, minimal_iff_forall_ssubset.2 ⟨⟨?_, h'.isSumFlat_union⟩, ?_⟩⟩
 
-  -- have := hN.isModularPair.inter_closure_eq
-  -- -- have hmod := (hN _ (N.closure_isFlat (F₁ ∪ M.closure (insert e F₀)))).inter_closure_eq
-  -- rw [closure_closure] at hmod
-  -- grw [← inter_eq_self_of_subset_left (N.closure_subset_ground _), inter_assoc, inter_comm N.E,
-  --   N.subset_closure (M.E ∩ N.E), ← hmod]
-  -- have hmod' := (hN F₁ h.isFlat_right).inter_closure_eq
-  -- rw [← inter_assoc, closure_inter_ground] at hmod
+--   -- have := hN.isModularPair.inter_closure_eq
+--   -- -- have hmod := (hN _ (N.closure_isFlat (F₁ ∪ M.closure (insert e F₀)))).inter_closure_eq
+--   -- rw [closure_closure] at hmod
+--   -- grw [← inter_eq_self_of_subset_left (N.closure_subset_ground _), inter_assoc, inter_comm N.E,
+--   --   N.subset_closure (M.E ∩ N.E), ← hmod]
+--   -- have hmod' := (hN F₁ h.isFlat_right).inter_closure_eq
+--   -- rw [← inter_assoc, closure_inter_ground] at hmod
 
-    -- have := h.subset_right
+--     -- have := h.subset_right
 
--- lemma foo (hM : M.IsFlat F₀) (hN : N.IsFlat F₁) (hF₀F₁ : F₁ ∩ M.E ⊆ F₀) (heM : e ∈ M.E) (heN : e ∉ N.E) (heF₀ : e ∉ F₀) :
---     N.closure (F₁ ∪ (M.closure (insert e F₀) ∩ N.E)) ∩ M.E ⊆ M.closure (insert e F₀)
+-- -- lemma foo (hM : M.IsFlat F₀) (hN : N.IsFlat F₁) (hF₀F₁ : F₁ ∩ M.E ⊆ F₀) (heM : e ∈ M.E) (heN : e ∉ N.E) (heF₀ : e ∉ F₀) :
+-- --     N.closure (F₁ ∪ (M.closure (insert e F₀) ∩ N.E)) ∩ M.E ⊆ M.closure (insert e F₀)
 
--- lemma sumFlat'_iInter (M N : Matroid α) [Nonempty ι] (F₀ F₁ F : ι → Set α)
---     (h : ∀ i, SumFlat' M N (F₀ i) (F₁ i) (F i)) :
---     SumFlat' M N (⋂ i, F₀ i) (⋂ i, F₁ i) (⋂ i, F i) := by
---   refine ⟨IsFlat.iInter (fun i ↦ (h i).isFlat_left), IsFlat.iInter (fun i ↦ (h i).isFlat_right),
---     ?_, ?_, ?_⟩
---   · rw [iInter_inter, iInter_congr fun i ↦ (h i).inter_left]
---   · rw [iInter_inter, iInter_congr fun i ↦ (h i).inter_right]
---   obtain i : ι := Classical.ofNonempty
---   grw [← iInter_congr (fun i ↦ (h i).inter_left), ← iInter_congr (fun i ↦ (h i).inter_right),
---     ← iInter_inter, ← iInter_inter, ← inter_union_distrib_left, inter_eq_left,
---     iInter_subset _ i, ← (h i).union_eq]
---   exact union_subset_union (h i).isFlat_left.subset_ground (h i).isFlat_right.subset_ground
+-- -- lemma sumFlat'_iInter (M N : Matroid α) [Nonempty ι] (F₀ F₁ F : ι → Set α)
+-- --     (h : ∀ i, SumFlat' M N (F₀ i) (F₁ i) (F i)) :
+-- --     SumFlat' M N (⋂ i, F₀ i) (⋂ i, F₁ i) (⋂ i, F i) := by
+-- --   refine ⟨IsFlat.iInter (fun i ↦ (h i).isFlat_left), IsFlat.iInter (fun i ↦ (h i).isFlat_right),
+-- --     ?_, ?_, ?_⟩
+-- --   · rw [iInter_inter, iInter_congr fun i ↦ (h i).inter_left]
+-- --   · rw [iInter_inter, iInter_congr fun i ↦ (h i).inter_right]
+-- --   obtain i : ι := Classical.ofNonempty
+-- --   grw [← iInter_congr (fun i ↦ (h i).inter_left), ← iInter_congr (fun i ↦ (h i).inter_right),
+-- --     ← iInter_inter, ← iInter_inter, ← inter_union_distrib_left, inter_eq_left,
+-- --     iInter_subset _ i, ← (h i).union_eq]
+-- --   exact union_subset_union (h i).isFlat_left.subset_ground (h i).isFlat_right.subset_ground
 
--- lemma SumFlat'.bar_left (hF : SumFlat' M N F₀ F₁ F) (heM : e ∈ M.E) (he : e ∉ N.E) (heF : e ∉ F₀) :
---   SumFlat M N (M.closure (insert e F₀)) (N.closure (F₁ ∪ (M.closure (insert e F₀) ∩ N.E)))
+-- -- lemma SumFlat'.bar_left (hF : SumFlat' M N F₀ F₁ F) (heM : e ∈ M.E) (he : e ∉ N.E) (heF : e ∉ F₀) :
+-- --   SumFlat M N (M.closure (insert e F₀)) (N.closure (F₁ ∪ (M.closure (insert e F₀) ∩ N.E)))
 
--- lemma sumFlat_ground (M N : Matroid α) : SumFlat M N (M.E ∪ N.E) := by
---   refine ⟨?_, ?_, rfl.subset⟩
---   · rw [inter_eq_self_of_subset_right subset_union_left]
---     exact M.ground_isFlat
---   rw [inter_eq_self_of_subset_right subset_union_right]
---   exact N.ground_isFlat
+-- -- lemma sumFlat_ground (M N : Matroid α) : SumFlat M N (M.E ∪ N.E) := by
+-- --   refine ⟨?_, ?_, rfl.subset⟩
+-- --   · rw [inter_eq_self_of_subset_right subset_union_left]
+-- --     exact M.ground_isFlat
+-- --   rw [inter_eq_self_of_subset_right subset_union_right]
+-- --   exact N.ground_isFlat
 
--- lemma sumFlat_iInter [Nonempty ι] (F : ι → Set α) (hFs : ∀ i, SumFlat M N (F i)) :
---     SumFlat M N <| (⋂ i, F i) := by
---   refine ⟨?_, ?_, ?_⟩
---   · rw [iInter_inter]
---     exact IsFlat.iInter fun i ↦ (hFs i).isFlat_left
---   · rw [iInter_inter]
---     exact IsFlat.iInter fun i ↦ (hFs i).isFlat_right
---   sorry
-
-
--- lemma SumFlat.inter (hF : SumFlat M N F) (hF' : SumFlat M N F') :
---     SumFlat M N (F ∩ F') := sorry
-
--- -- @[simp]
--- lemma sumFlat_closure_union_closure (hX : M.closure X ∩ N.E ⊆ N.closure Y)
---     (hY : N.closure Y ∩ M.E ⊆ M.closure X) : SumFlat M N (M.closure X ∪ N.closure Y) := by
---   refine ⟨?_, ?_, union_subset_union (closure_subset_ground ..) (closure_subset_ground ..)⟩
---   · rw [union_inter_distrib_right, union_eq_self_of_subset_right (by grind),
---       inter_eq_self_of_subset_left (M.closure_subset_ground ..)]
---     exact M.closure_isFlat ..
---   rw [union_inter_distrib_right, inter_eq_self_of_subset_left (N.closure_subset_ground ..),
---     union_eq_self_of_subset_left hX]
---   exact N.closure_isFlat ..
+-- -- lemma sumFlat_iInter [Nonempty ι] (F : ι → Set α) (hFs : ∀ i, SumFlat M N (F i)) :
+-- --     SumFlat M N <| (⋂ i, F i) := by
+-- --   refine ⟨?_, ?_, ?_⟩
+-- --   · rw [iInter_inter]
+-- --     exact IsFlat.iInter fun i ↦ (hFs i).isFlat_left
+-- --   · rw [iInter_inter]
+-- --     exact IsFlat.iInter fun i ↦ (hFs i).isFlat_right
+-- --   sorry
 
 
--- lemma SumFlat.bar_left (hF : SumFlat M N F) (heM : e ∈ M.E) (he : e ∉ N.E) (heF : e ∉ F) :
---   SumFlat M N (M.closure (insert e (F ∩ M.E)) ∪ N.closure (F ∩ N.E ∪ N.closure ((insert e (F ∩ M.E)))))
+-- -- lemma SumFlat.inter (hF : SumFlat M N F) (hF' : SumFlat M N F') :
+-- --     SumFlat M N (F ∩ F') := sorry
 
--- lemma SumFlat.foo_left (hF : SumFlat M N F) (heM : e ∈ M.E) (he : e ∉ N.E) (heF : e ∉ F) :
---     ∃ F', SumFlat M N F' ∧ e ∈ F' ∧ Minimal (fun X ↦ F ⊂ X ∧ SumFlat M N X) F' := by
---   have hsf : SumFlat M N
---       (M.closure (insert e (F ∩ M.E)) ∪ N.closure ((F ∩ M.closure (F ∩ M.E ∩ N.E)) ∩ N.E)) := by
---     refine sumFlat_closure_union_closure ?_ ?_
---   refine ⟨_, hsf,
---     .inl (mem_closure_of_mem' _ (mem_insert ..) he), minimal_iff_forall_ssubset.2
---     ⟨⟨?_, hsf⟩, ?_⟩⟩
+-- -- -- @[simp]
+-- -- lemma sumFlat_closure_union_closure (hX : M.closure X ∩ N.E ⊆ N.closure Y)
+-- --     (hY : N.closure Y ∩ M.E ⊆ M.closure X) : SumFlat M N (M.closure X ∪ N.closure Y) := by
+-- --   refine ⟨?_, ?_, union_subset_union (closure_subset_ground ..) (closure_subset_ground ..)⟩
+-- --   · rw [union_inter_distrib_right, union_eq_self_of_subset_right (by grind),
+-- --       inter_eq_self_of_subset_left (M.closure_subset_ground ..)]
+-- --     exact M.closure_isFlat ..
+-- --   rw [union_inter_distrib_right, inter_eq_self_of_subset_left (N.closure_subset_ground ..),
+-- --     union_eq_self_of_subset_left hX]
+-- --   exact N.closure_isFlat ..
 
---   · sorry
---   sorry
+
+-- -- lemma SumFlat.bar_left (hF : SumFlat M N F) (heM : e ∈ M.E) (he : e ∉ N.E) (heF : e ∉ F) :
+-- --   SumFlat M N (M.closure (insert e (F ∩ M.E)) ∪ N.closure (F ∩ N.E ∪ N.closure ((insert e (F ∩ M.E)))))
+
+-- -- lemma SumFlat.foo_left (hF : SumFlat M N F) (heM : e ∈ M.E) (he : e ∉ N.E) (heF : e ∉ F) :
+-- --     ∃ F', SumFlat M N F' ∧ e ∈ F' ∧ Minimal (fun X ↦ F ⊂ X ∧ SumFlat M N X) F' := by
+-- --   have hsf : SumFlat M N
+-- --       (M.closure (insert e (F ∩ M.E)) ∪ N.closure ((F ∩ M.closure (F ∩ M.E ∩ N.E)) ∩ N.E)) := by
+-- --     refine sumFlat_closure_union_closure ?_ ?_
+-- --   refine ⟨_, hsf,
+-- --     .inl (mem_closure_of_mem' _ (mem_insert ..) he), minimal_iff_forall_ssubset.2
+-- --     ⟨⟨?_, hsf⟩, ?_⟩⟩
+
+-- --   · sorry
+-- --   sorry
 
 
 
 
 
--- lemma SumFlat.foo (hF : SumFlat M N F) (he : e ∈ M.E ∪ N.E) (heF : e ∉ F) :
---     ∃! F', SumFlat M N F' ∧ e ∈ F' ∧ Minimal (fun X ↦ F ⊂ X ∧ SumFlat M N X) F' := by
---   sorry
+-- -- lemma SumFlat.foo (hF : SumFlat M N F) (he : e ∈ M.E ∪ N.E) (heF : e ∉ F) :
+-- --     ∃! F', SumFlat M N F' ∧ e ∈ F' ∧ Minimal (fun X ↦ F ⊂ X ∧ SumFlat M N X) F' := by
+-- --   sorry
 
---     -- rw [inter_assoc, inter_eq_self_of_subset_right subset_union_left]
---     -- have := IsFlat.iInter_inter_ground (M := M) (Fs := fun (F : Fs) ↦ F.1 ∩ M.E)
---     --   (fun F ↦ (hFs F.1 F.2).isFlat_left)
---     -- simp only [iInter_coe_set] at this
---     -- rw [biInter_inter] at this
+-- --     -- rw [inter_assoc, inter_eq_self_of_subset_right subset_union_left]
+-- --     -- have := IsFlat.iInter_inter_ground (M := M) (Fs := fun (F : Fs) ↦ F.1 ∩ M.E)
+-- --     --   (fun F ↦ (hFs F.1 F.2).isFlat_left)
+-- --     -- simp only [iInter_coe_set] at this
+-- --     -- rw [biInter_inter] at this
